myMap.v
@@ -83,7 +83,7 @@ Proof.
               (fold_right (F A f) neutral
                  (MapFold1 A (alist A) (anil A) (aapp A)
                     (fun (a : ad) (y : A) => acons A (a, y) (anil A))
-                    (fun a0 : ad => pf (Ndouble a0)) m0))
+                    (fun a0 : ad => pf (N.double a0)) m0))
               (fold_right (F A f) neutral
                  (MapFold1 A (alist A) (anil A) (aapp A)
                     (fun (a : ad) (y : A) => acons A (a, y) (anil A))
@@ -171,7 +171,7 @@ Lemma my_alist_of_map_lemma_1 :
 Proof.
   intros A m a y.  rewrite (alist_of_Map_semantics _ m a).
   generalize (alist_of_Map A m).  simple induction a0.  simpl in |- *.  intro; discriminate.
-  simpl in |- *.  intro a1.  elim a1.  intros a2 b l H H0.  elim (sumbool_of_bool (Neqb a2 a)).
+  simpl in |- *.  intro a1.  elim a1.  intros a2 b l H H0.  elim (sumbool_of_bool (N.eqb a2 a)).
   intro H1.  left.  rewrite H1 in H0.  injection H0; intro H2.  rewrite H2.
   rewrite (Neqb_complete _ _ H1).  reflexivity.  intro H1.  rewrite H1 in H0.
   right.  apply H.  assumption.
@@ -193,40 +193,40 @@ Proof.
    (in_app_or
       (MapFold1 A (list (ad * A)) (anil A) (app (A:=ad * A))
          (fun (a0 : ad) (y0 : A) => acons A (a0, y0) (anil A))
-         (fun a0 : ad => pf (Ndouble a0)) m0)
+         (fun a0 : ad => pf (N.double a0)) m0)
       (MapFold1 A (list (ad * A)) (anil A) (app (A:=ad * A))
          (fun (a0 : ad) (y0 : A) => acons A (a0, y0) (anil A))
          (fun a0 : ad => pf (Ndouble_plus_one a0)) m1) 
       (a, y) H2).
   intro H3.  fold (aapp A) in H3.  rewrite (MapGet_M2_bit_0_if A m0 m1 (fp a)).
-  cut (forall a : ad, Ndiv2 (fp (pf (Ndouble a))) = a).
+  cut (forall a : ad, N.div2 (fp (pf (N.double a))) = a).
   intro H4.  elim
-   (H (fun a0 : ad => pf (Ndouble a0)) (fun a0 : ad => Ndiv2 (fp a0)) H4
+   (H (fun a0 : ad => pf (N.double a0)) (fun a0 : ad => N.div2 (fp a0)) H4
       a y H3).
   intros H5 H6.  elim (sumbool_of_bool (Nbit0 (fp a))).  intro H7.
-  cut (Neqb (Ndouble (Ndiv2 (fp a))) (fp a) = false).  intro H8.
-  cut (fp (pf (Ndouble (Ndiv2 (fp a)))) = fp a).  rewrite (H1 (Ndouble (Ndiv2 (fp a)))).
+  cut (N.eqb (N.double (N.div2 (fp a))) (fp a) = false).  intro H8.
+  cut (fp (pf (N.double (N.div2 (fp a)))) = fp a).  rewrite (H1 (N.double (N.div2 (fp a)))).
   intro H9.  rewrite H9 in H8.  rewrite (Neqb_correct (fp a)) in H8.  discriminate.
   rewrite H6.  reflexivity.  apply Nodd_not_double.  assumption.  intro H7.
   rewrite H7.  cut
-   (MapGet A m0 ((fun a0 : ad => Ndiv2 (fp a0)) a) = Some y /\
-    (fun a0 : ad => pf (Ndouble a0)) ((fun a0 : ad => Ndiv2 (fp a0)) a) =
+   (MapGet A m0 ((fun a0 : ad => N.div2 (fp a0)) a) = Some y /\
+    (fun a0 : ad => pf (N.double a0)) ((fun a0 : ad => N.div2 (fp a0)) a) =
     a).
-  intro H8.  split.  exact (proj1 H8).  replace (fp a) with (fp (pf (Ndouble (Ndiv2 (fp a))))).
-  rewrite (H1 (Ndouble (Ndiv2 (fp a)))).  assumption.  rewrite (proj2 H8).
+  intro H8.  split.  exact (proj1 H8).  replace (fp a) with (fp (pf (N.double (N.div2 (fp a))))).
+  rewrite (H1 (N.double (N.div2 (fp a)))).  assumption.  rewrite (proj2 H8).
   reflexivity.  exact
-   (H (fun a0 : ad => pf (Ndouble a0)) (fun a0 : ad => Ndiv2 (fp a0)) H4
+   (H (fun a0 : ad => pf (N.double a0)) (fun a0 : ad => N.div2 (fp a0)) H4
       a y H3).
-  intro a0.  rewrite (H1 (Ndouble a0)).  apply Ndouble_div2.  intro H3.
+  intro a0.  rewrite (H1 (N.double a0)).  apply Ndouble_div2.  intro H3.
   fold (aapp A) in H3.  rewrite (MapGet_M2_bit_0_if A m0 m1 (fp a)).
-  cut (forall a : ad, Ndiv2 (fp (pf (Ndouble_plus_one a))) = a).
+  cut (forall a : ad, N.div2 (fp (pf (Ndouble_plus_one a))) = a).
   intro H4.  elim
    (H0 (fun a0 : ad => pf (Ndouble_plus_one a0))
-      (fun a0 : ad => Ndiv2 (fp a0)) H4 a y H3).
+      (fun a0 : ad => N.div2 (fp a0)) H4 a y H3).
   intros H5 H6.  elim (sumbool_of_bool (Nbit0 (fp a))).  intro H7.  rewrite H7.
   split.  assumption.  rewrite (Ndiv2_double_plus_one (fp a) H7) in H6.
-  assumption.  intro H7.  cut (Neqb (Ndouble_plus_one (Ndiv2 (fp a))) (fp a) = false).
-  cut (fp (pf (Ndouble_plus_one (Ndiv2 (fp a)))) = fp a).  rewrite (H1 (Ndouble_plus_one (Ndiv2 (fp a)))).
+  assumption.  intro H7.  cut (N.eqb (Ndouble_plus_one (N.div2 (fp a))) (fp a) = false).
+  cut (fp (pf (Ndouble_plus_one (N.div2 (fp a)))) = fp a).  rewrite (H1 (Ndouble_plus_one (N.div2 (fp a)))).
   intros H8 H9.  rewrite H8 in H9.  rewrite (Neqb_correct (fp a)) in H9.  discriminate.
   rewrite H6.  reflexivity.  apply Neven_not_double_plus_one.  assumption.
   intro a0.  rewrite (H1 (Ndouble_plus_one a0)).  apply Ndouble_plus_one_div2.
@@ -396,15 +396,15 @@ Definition MapPut3 (m : Map (Map (Map A))) (a b c : ad)
 Lemma MapPut2_semantics :
  forall (m : Map (Map A)) (a b a1 b1 : ad) (c : A),
  MapGet2 (MapPut2 m a b c) a1 b1 =
- (if Neqb a a1 && Neqb b b1 then Some c else MapGet2 m a1 b1).
+ (if N.eqb a a1 && N.eqb b b1 then Some c else MapGet2 m a1 b1).
 Proof.
   intros m a b a1 b1 c.  unfold MapGet2, MapPut2 in |- *.  elim (option_sum _ (MapGet (Map A) m a)).
   intro H.  elim H; clear H; intros x H.  rewrite H.
   rewrite (MapPut_semantics (Map A) m a (MapPut A x b c) a1).
-  elim (sumbool_of_bool (Neqb a a1)).  intro H0.  rewrite H0.  simpl in |- *.
+  elim (sumbool_of_bool (N.eqb a a1)).  intro H0.  rewrite H0.  simpl in |- *.
   rewrite (MapPut_semantics A x b c b1).  rewrite <- (Neqb_complete a a1).
   rewrite H.  reflexivity.  assumption.  intro H0.  rewrite H0.  simpl in |- *.
-  reflexivity.  intro H.  rewrite H.  simpl in |- *.  elim (sumbool_of_bool (Neqb a a1)).
+  reflexivity.  intro H.  rewrite H.  simpl in |- *.  elim (sumbool_of_bool (N.eqb a a1)).
   intro H0.  rewrite H0.  simpl in |- *.
   rewrite (MapPut_semantics (Map A) m a (M1 A b c) a1).  rewrite H0.  simpl in |- *.
   rewrite <- (Neqb_complete _ _ H0).  rewrite H.  reflexivity.  intro H0.
@@ -415,7 +415,7 @@ Qed.
 Lemma MapPut3_semantics :
  forall (m : Map (Map (Map A))) (a b c a1 b1 c1 : ad) (d : A),
  MapGet3 (MapPut3 m a b c d) a1 b1 c1 =
- (if Neqb a a1 && (Neqb b b1 && Neqb c c1)
+ (if N.eqb a a1 && (N.eqb b b1 && N.eqb c c1)
   then Some d
   else MapGet3 m a1 b1 c1).
 Proof.
@@ -423,13 +423,13 @@ Proof.
   elim (option_sum _ (MapGet (Map (Map A)) m a)).  intro H.
   elim H; clear H; intros x H.  rewrite H.
   rewrite (MapPut_semantics (Map (Map A)) m a (MapPut2 x b c d) a1).
-  elim (sumbool_of_bool (Neqb a a1)).  intro H0.  rewrite H0.  simpl in |- *.
+  elim (sumbool_of_bool (N.eqb a a1)).  intro H0.  rewrite H0.  simpl in |- *.
   rewrite <- (Neqb_complete _ _ H0).  rewrite (MapPut2_semantics x b c b1 c1 d).
   rewrite H.  reflexivity.  intro H0.  rewrite H0.  simpl in |- *.  reflexivity.  intro H.
   rewrite H.  rewrite (MapPut_semantics (Map (Map A)) m a (M1 (Map A) b (M1 A c d)) a1).
-  elim (sumbool_of_bool (Neqb a a1)).  intro H0.  rewrite H0.  simpl in |- *.
+  elim (sumbool_of_bool (N.eqb a a1)).  intro H0.  rewrite H0.  simpl in |- *.
   unfold MapGet2 in |- *.  simpl in |- *.  rewrite <- (Neqb_complete _ _ H0).  rewrite H.
-  elim (Neqb b b1).  simpl in |- *.  reflexivity.  simpl in |- *.  reflexivity.  intro H0.
+  elim (N.eqb b b1).  simpl in |- *.  reflexivity.  simpl in |- *.  reflexivity.  intro H0.
   rewrite H0.  simpl in |- *.  reflexivity.
 Qed.
 
@@ -502,7 +502,7 @@ Fixpoint map_app_list1 (pf : ad -> ad) (l : list ad)
   | M1 a y => pf a :: l
   | M2 m1 m2 =>
       map_app_list1 (fun a0 : ad => pf (Ndouble_plus_one a0))
-        (map_app_list1 (fun a0 : ad => pf (Ndouble a0)) l m1) m2
+        (map_app_list1 (fun a0 : ad => pf (N.double a0)) l m1) m2
   end.
 
 Lemma map_app_list1_lemma_1 :
@@ -524,27 +524,27 @@ Proof.
   elim H0; intro H2.  rewrite <- H2.  rewrite (H a).  right.  unfold in_dom in |- *.
   simpl in |- *.  rewrite (Neqb_correct a).  split; reflexivity.  left; assumption.
   simpl in |- *.  intros m0 H m1 H0 pf fp l H1 a H2.
-  cut (forall a : ad, Ndiv2 (fp (pf (Ndouble_plus_one a))) = a).
+  cut (forall a : ad, N.div2 (fp (pf (Ndouble_plus_one a))) = a).
   intro H3.  elim
    (H0 (fun a0 : ad => pf (Ndouble_plus_one a0))
-      (fun a0 : ad => Ndiv2 (fp a0)) _ H3 a H2).
+      (fun a0 : ad => N.div2 (fp a0)) _ H3 a H2).
   intro H4.
-  cut (forall a : ad, Ndiv2 (fp (pf (Ndouble a))) = a).
+  cut (forall a : ad, N.div2 (fp (pf (N.double a))) = a).
   intro H5.  elim
-   (H (fun a0 : ad => pf (Ndouble a0)) (fun a0 : ad => Ndiv2 (fp a0)) _
+   (H (fun a0 : ad => pf (N.double a0)) (fun a0 : ad => N.div2 (fp a0)) _
       H5 a H4).
   tauto.  intro H6.  elim H6; clear H6; intros H6 H7.  right.
   elim (sumbool_of_bool (Nbit0 (fp a))).  intro y.  rewrite <- H7 in y.
-  rewrite (H1 (Ndouble (Ndiv2 (fp a)))) in y.  rewrite (Ndouble_bit0 (Ndiv2 (fp a))) in y.
+  rewrite (H1 (N.double (N.div2 (fp a)))) in y.  rewrite (Ndouble_bit0 (N.div2 (fp a))) in y.
   discriminate.  intro y.  unfold in_dom in |- *.  rewrite (MapGet_M2_bit_0_0 _ (fp a) y m0 m1).
   unfold in_dom in H6.  split.  assumption.  rewrite (Ndiv2_double (fp a) y) in H7.
-  assumption.  intro a0.  rewrite (H1 (Ndouble a0)).  apply Ndouble_div2.
+  assumption.  intro a0.  rewrite (H1 (N.double a0)).  apply Ndouble_div2.
   intro H4.  elim H4; clear H4; intros H4 H5.  right.
   elim (sumbool_of_bool (Nbit0 (fp a))).  intro y.  unfold in_dom in |- *.
   rewrite (MapGet_M2_bit_0_1 _ (fp a) y m0 m1).  unfold in_dom in H4.  split.
   assumption.  rewrite (Ndiv2_double_plus_one _ y) in H5.  assumption.  intro y.
-  rewrite <- H5 in y.  rewrite (H1 (Ndouble_plus_one (Ndiv2 (fp a)))) in y.
-  rewrite (Ndouble_plus_one_bit0 (Ndiv2 (fp a))) in y.  discriminate.
+  rewrite <- H5 in y.  rewrite (H1 (Ndouble_plus_one (N.div2 (fp a)))) in y.
+  rewrite (Ndouble_plus_one_bit0 (N.div2 (fp a))) in y.  discriminate.
   intro a0.  rewrite (H1 (Ndouble_plus_one a0)).  apply Ndouble_plus_one_div2.
 Qed.
 
@@ -558,27 +558,27 @@ Proof.
   simple induction m.  simpl in |- *.  tauto.  simpl in |- *.  intros a a0 pf fp l H H0 H1.  apply no_dup_cons.  unfold not in |- *.
   intro H2.  absurd (In (pf a) l).  apply H1 with (a1 := a).  unfold in_dom in |- *.  simpl in |- *.
   rewrite (Neqb_correct a).  reflexivity.  assumption.  assumption.  simpl in |- *.
-  intros m0 H m1 H0 pf fp l H1 H2 H3.  apply H0 with (fp := fun a0 : ad => Ndiv2 (fp a0)).  intro a0.
+  intros m0 H m1 H0 pf fp l H1 H2 H3.  apply H0 with (fp := fun a0 : ad => N.div2 (fp a0)).  intro a0.
   rewrite (H1 (Ndouble_plus_one a0)).  apply Ndouble_plus_one_div2.
-  apply H with (fp := fun a0 : ad => Ndiv2 (fp a0)).  intro a0.  rewrite (H1 (Ndouble a0)).
+  apply H with (fp := fun a0 : ad => N.div2 (fp a0)).  intro a0.  rewrite (H1 (N.double a0)).
   apply Ndouble_div2.  assumption.  intros a H4.  apply H3.  unfold in_dom in |- *.
-  rewrite (MapGet_M2_bit_0_0 _ (Ndouble a) (Ndouble_bit0 _) m0 m1).
+  rewrite (MapGet_M2_bit_0_0 _ (N.double a) (Ndouble_bit0 _) m0 m1).
   rewrite (Ndouble_div2 a).  assumption.  intros a H4.  unfold not in |- *; intro H5.
-  cut (forall a : ad, Ndiv2 (fp (pf (Ndouble a))) = a).
+  cut (forall a : ad, N.div2 (fp (pf (N.double a))) = a).
   intro H6.  elim
-   (map_app_list1_lemma_2 m0 (fun a0 : ad => pf (Ndouble a0))
-      (fun a0 : ad => Ndiv2 (fp a0)) l H6 _ H5).
+   (map_app_list1_lemma_2 m0 (fun a0 : ad => pf (N.double a0))
+      (fun a0 : ad => N.div2 (fp a0)) l H6 _ H5).
   unfold not in H3.  intro H7.  apply H3 with (a := Ndouble_plus_one a).
   unfold in_dom in |- *.  rewrite
    (MapGet_M2_bit_0_1 _ (Ndouble_plus_one a) (Ndouble_plus_one_bit0 _) m0
       m1).
   rewrite (Ndouble_plus_one_div2 a).  assumption.  assumption.  intro H7.
   elim H7; clear H7; intros H7 H8.  rewrite (H1 (Ndouble_plus_one a)) in H8.
-  rewrite (Ndouble_plus_one_div2 a) in H8.  elim (sumbool_of_bool (Nbit0 (Ndouble a))).
+  rewrite (Ndouble_plus_one_div2 a) in H8.  elim (sumbool_of_bool (Nbit0 (N.double a))).
   intro y.  rewrite (Ndouble_bit0 a) in y.  discriminate.  intro y.
-  rewrite <- (H1 (Ndouble a)) in y.  rewrite H8 in y.
+  rewrite <- (H1 (N.double a)) in y.  rewrite H8 in y.
   rewrite (H1 (Ndouble_plus_one a)) in y.  rewrite (Ndouble_plus_one_bit0 a) in y.
-  discriminate.  intro a0.  rewrite (H1 (Ndouble a0)).  apply Ndouble_div2.
+  discriminate.  intro a0.  rewrite (H1 (N.double a0)).  apply Ndouble_div2.
 Qed.
 
 Lemma map_app_list1_lemma_4 :
@@ -586,17 +586,17 @@ Lemma map_app_list1_lemma_4 :
  in_dom _ a m = true -> In (pf a) (map_app_list1 pf l m).
 Proof.
   simple induction m.  simpl in |- *.  unfold in_dom in |- *.  simpl in |- *.  intros; discriminate.  simpl in |- *.
-  intros.  unfold in_dom in H.  simpl in H.  elim (sumbool_of_bool (Neqb a a1)).
+  intros.  unfold in_dom in H.  simpl in H.  elim (sumbool_of_bool (N.eqb a a1)).
   intro y.  rewrite y in H.  rewrite (Neqb_complete _ _ y).  left.  reflexivity.
   intro y.  rewrite y in H.  discriminate.  simpl in |- *.  intros.
   elim (sumbool_of_bool (Nbit0 a)).  intro y.  unfold in_dom in H1.
   rewrite (MapGet_M2_bit_0_1 _ a y m0 m1) in H1.
   replace (pf a) with
-   ((fun a0 : ad => pf (Ndouble_plus_one a0)) (Ndiv2 a)).
+   ((fun a0 : ad => pf (Ndouble_plus_one a0)) (N.div2 a)).
   apply H0 with (pf := fun a0 : ad => pf (Ndouble_plus_one a0)).  assumption.  
   rewrite (Ndiv2_double_plus_one a).  reflexivity.  assumption.  intro y.
-  apply map_app_list1_lemma_1.  replace (pf a) with (pf (Ndouble (Ndiv2 a))).
-  apply H with (pf := fun a0 : ad => pf (Ndouble a0)).  unfold in_dom in |- *.
+  apply map_app_list1_lemma_1.  replace (pf a) with (pf (N.double (N.div2 a))).
+  apply H with (pf := fun a0 : ad => pf (N.double a0)).  unfold in_dom in |- *.
   unfold in_dom in H1.  rewrite (MapGet_M2_bit_0_0 _ _ y m0 m1) in H1.
   assumption.  rewrite (Ndiv2_double _ y).  reflexivity.  
 Qed.
@@ -618,7 +618,7 @@ Fixpoint MapDomRestrByApp1 (pf : ad -> ad) (l : list ad)
       | M1 a' y' => map_app_list1 pf l (MapRemove A m a')
       | M2 m'1 m'2 =>
           MapDomRestrByApp1 (fun a0 : ad => pf (Ndouble_plus_one a0))
-            (MapDomRestrByApp1 (fun a0 : ad => pf (Ndouble a0)) l m1 m'1)
+            (MapDomRestrByApp1 (fun a0 : ad => pf (N.double a0)) l m1 m'1)
             m2 m'2
       end
   end.
@@ -641,7 +641,7 @@ Lemma MapDomRestrByApp1_lemma_2 :
  in_dom _ a m' = false -> In (pf a) (MapDomRestrByApp1 pf l m m').
 Proof.
   simple induction m.  simpl in |- *.  unfold in_dom at 1 in |- *.  simpl in |- *.  intros.  discriminate.
-  unfold in_dom in |- *.  simpl in |- *.  intros.  elim (sumbool_of_bool (Neqb a a1)).  intro y.
+  unfold in_dom in |- *.  simpl in |- *.  intros.  elim (sumbool_of_bool (N.eqb a a1)).  intro y.
   rewrite (Neqb_complete _ _ y).  elim (option_sum _ (MapGet B m' a1)).  intro y0.
   inversion y0.  rewrite H1 in H0.  rewrite y in H.  discriminate.  intro y0.
   rewrite y0.  simpl in |- *.  left.  reflexivity.  intro y.  rewrite y in H.
@@ -650,19 +650,19 @@ Proof.
   unfold MapDomRestrByApp1 in |- *.  unfold in_dom in H2.  simpl in H2.
   apply map_app_list1_lemma_4.  unfold in_dom in |- *.
   rewrite (MapRemove_semantics A (M2 A m0 m1) a a1).
-  elim (sumbool_of_bool (Neqb a a1)).  intro y.  rewrite y in H2.  discriminate.
+  elim (sumbool_of_bool (N.eqb a a1)).  intro y.  rewrite y in H2.  discriminate.
   intro y.  rewrite y.  assumption.  intros.  simpl in |- *.
   elim (sumbool_of_bool (Nbit0 a)).  intro y.  unfold in_dom in H3, H4.
   rewrite (MapGet_M2_bit_0_1 A a y m0 m1) in H3.
   rewrite (MapGet_M2_bit_0_1 B a y m2 m3) in H4.
-  replace (pf a) with (pf (Ndouble_plus_one (Ndiv2 a))).
+  replace (pf a) with (pf (Ndouble_plus_one (N.div2 a))).
   apply H0 with (pf := fun a0 : ad => pf (Ndouble_plus_one a0)).  assumption.
   assumption.  rewrite (Ndiv2_double_plus_one _ y).  reflexivity.  intro y.
   unfold in_dom in H3, H4.  rewrite (MapGet_M2_bit_0_0 A a y m0 m1) in H3.
   rewrite (MapGet_M2_bit_0_0 B a y m2 m3) in H4.
   apply MapDomRestrByApp1_lemma_1.
-  replace (pf a) with (pf (Ndouble (Ndiv2 a))).
-  apply H with (pf := fun a0 : ad => pf (Ndouble a0)).  assumption.  assumption.  
+  replace (pf a) with (pf (N.double (N.div2 a))).
+  apply H with (pf := fun a0 : ad => pf (N.double a0)).  assumption.  assumption.  
   rewrite (Ndiv2_double _ y).  reflexivity.
 Qed.
 
@@ -687,22 +687,22 @@ Proof.
   elim (map_app_list1_lemma_2 _ _ _ _ H1 a1 H2).  tauto.  intro H3.
   elim H3; clear H3; intros.  right.  unfold in_dom in H3.
   rewrite (MapRemove_semantics A (M2 A m0 m1) a (fp a1)) in H3.
-  elim (sumbool_of_bool (Neqb a (fp a1))).  intro y.  rewrite y in H3.
+  elim (sumbool_of_bool (N.eqb a (fp a1))).  intro y.  rewrite y in H3.
   discriminate.  intro y.  rewrite y in H3.  split.  assumption.  split.
   unfold in_dom in |- *.  simpl in |- *.  rewrite y.  reflexivity.  assumption.  intros.
   simpl in H4.
-  cut (forall a : ad, Ndiv2 (fp (pf (Ndouble a))) = a).
-  cut (forall a : ad, Ndiv2 (fp (pf (Ndouble_plus_one a))) = a).
+  cut (forall a : ad, N.div2 (fp (pf (N.double a))) = a).
+  cut (forall a : ad, N.div2 (fp (pf (Ndouble_plus_one a))) = a).
   intros.  elim
    (H0 m3 _ (fun a0 : ad => pf (Ndouble_plus_one a0))
-      (fun a0 : ad => Ndiv2 (fp a0)) H5 _ H4).
+      (fun a0 : ad => N.div2 (fp a0)) H5 _ H4).
   intro.  elim
-   (H m2 _ (fun a0 : ad => pf (Ndouble a0))
-      (fun a0 : ad => Ndiv2 (fp a0)) H6 _ H7).
+   (H m2 _ (fun a0 : ad => pf (N.double a0))
+      (fun a0 : ad => N.div2 (fp a0)) H6 _ H7).
   tauto.  intro.  elim H8; clear H8; intros.  elim H9; clear H9; intros.
   right.  elim (sumbool_of_bool (Nbit0 (fp a))).  intro y.
-  rewrite <- H10 in y.  rewrite (H3 (Ndouble (Ndiv2 (fp a)))) in y.
-  rewrite (Ndouble_bit0 (Ndiv2 (fp a))) in y.  discriminate.  intro y.
+  rewrite <- H10 in y.  rewrite (H3 (N.double (N.div2 (fp a)))) in y.
+  rewrite (Ndouble_bit0 (N.div2 (fp a))) in y.  discriminate.  intro y.
   unfold in_dom in |- *.  rewrite (MapGet_M2_bit_0_0 _ _ y m0 m1).
   rewrite (MapGet_M2_bit_0_0 _ _ y m2 m3).  split.  assumption.  split.
   assumption.  rewrite (Ndiv2_double _ y) in H10.  assumption.  intro.
@@ -711,10 +711,10 @@ Proof.
   rewrite (MapGet_M2_bit_0_1 _ _ y m0 m1).  rewrite (MapGet_M2_bit_0_1 _ _ y m2 m3).
   split.  assumption.  split.  assumption.  rewrite (Ndiv2_double_plus_one _ y) in H9.
   assumption.  intro y.  rewrite <- H9 in y.
-  rewrite (H3 (Ndouble_plus_one (Ndiv2 (fp a)))) in y.
-  rewrite (Ndouble_plus_one_bit0 (Ndiv2 (fp a))) in y.  discriminate.  
+  rewrite (H3 (Ndouble_plus_one (N.div2 (fp a)))) in y.
+  rewrite (Ndouble_plus_one_bit0 (N.div2 (fp a))) in y.  discriminate.  
   intros.  rewrite (H3 (Ndouble_plus_one a0)).  apply Ndouble_plus_one_div2.
-  intros.  rewrite (H3 (Ndouble a0)).  apply Ndouble_div2.
+  intros.  rewrite (H3 (N.double a0)).  apply Ndouble_div2.
 Qed.
 
 Lemma MapDomRestrByApp1_lemma_4 :
@@ -734,19 +734,19 @@ Proof.
   intros.  unfold MapDomRestrByApp1 in |- *.  apply map_app_list1_lemma_3 with (fp := fp).
   assumption.  assumption.  intros.  apply H2.  unfold in_dom in |- *.
   unfold in_dom in H4.  rewrite (MapRemove_semantics A (M2 A m0 m1) a a1) in H4.
-  elim (sumbool_of_bool (Neqb a a1)).  intro y.  rewrite y in H4.  discriminate.
+  elim (sumbool_of_bool (N.eqb a a1)).  intro y.  rewrite y in H4.  discriminate.
   intro y.  rewrite y in H4.  assumption.  unfold in_dom in H4.
   rewrite (MapRemove_semantics A (M2 A m0 m1) a a1) in H4.
-  elim (sumbool_of_bool (Neqb a a1)).  intro y.  rewrite y in H4.  discriminate.
+  elim (sumbool_of_bool (N.eqb a a1)).  intro y.  rewrite y in H4.  discriminate.
   intro y.  rewrite y in H4.  unfold in_dom in |- *.  simpl in |- *.  rewrite y.  reflexivity.
   intros.  simpl in |- *.
-  cut (forall a : ad, Ndiv2 (fp (pf (Ndouble a))) = a).
-  cut (forall a : ad, Ndiv2 (fp (pf (Ndouble_plus_one a))) = a).
-  intros.  apply H0 with (fp := fun a0 : ad => Ndiv2 (fp a0)).  intro.
+  cut (forall a : ad, N.div2 (fp (pf (N.double a))) = a).
+  cut (forall a : ad, N.div2 (fp (pf (Ndouble_plus_one a))) = a).
+  intros.  apply H0 with (fp := fun a0 : ad => N.div2 (fp a0)).  intro.
   rewrite (H3 (Ndouble_plus_one a)).  apply Ndouble_plus_one_div2.  intros.
   unfold not in |- *.  intro.  elim
-   (MapDomRestrByApp1_lemma_3 m0 m2 l (fun a0 : ad => pf (Ndouble a0))
-      (fun a0 : ad => Ndiv2 (fp a0)) H7 (pf (Ndouble_plus_one a)) H10).
+   (MapDomRestrByApp1_lemma_3 m0 m2 l (fun a0 : ad => pf (N.double a0))
+      (fun a0 : ad => N.div2 (fp a0)) H7 (pf (Ndouble_plus_one a)) H10).
   intro.  unfold not in H4.  apply H4 with (a := Ndouble_plus_one a).
   unfold in_dom in |- *.  rewrite (MapGet_M2_bit_0_1 _ _ (Ndouble_plus_one_bit0 a) m0 m1).
   rewrite (Ndouble_plus_one_div2 a).  assumption.  unfold in_dom in |- *.
@@ -754,16 +754,16 @@ Proof.
   rewrite (Ndouble_plus_one_div2 a).  assumption.  assumption.  intros.
   elim H11; clear H11; intros.  elim H12; clear H12; intros.
   rewrite (H3 (Ndouble_plus_one a)) in H13.  rewrite (Ndouble_plus_one_div2 a) in H13.
-  cut (Ndouble a = Ndouble_plus_one a).  intros.  elim (sumbool_of_bool (Nbit0 (Ndouble a))).
+  cut (N.double a = Ndouble_plus_one a).  intros.  elim (sumbool_of_bool (Nbit0 (N.double a))).
   intro y.  rewrite (Ndouble_bit0 a) in y.  discriminate.  rewrite H14.
   rewrite (Ndouble_plus_one_bit0 a).  intro.  discriminate.  
-  rewrite <- (H3 (Ndouble a)).  rewrite H13.  apply H3.  
-  apply H with (fp := fun a0 : ad => Ndiv2 (fp a0)).  assumption.  intros.  apply H4.
+  rewrite <- (H3 (N.double a)).  rewrite H13.  apply H3.  
+  apply H with (fp := fun a0 : ad => N.div2 (fp a0)).  assumption.  intros.  apply H4.
   unfold in_dom in |- *.  rewrite (MapGet_M2_bit_0_0 _ _ (Ndouble_bit0 a) m0 m1).
   rewrite (Ndouble_div2 a).  assumption.  unfold in_dom in |- *.
   rewrite (MapGet_M2_bit_0_0 _ _ (Ndouble_bit0 a) m2 m3).  rewrite (Ndouble_div2 a).
   assumption.  assumption.  intros.  rewrite (H3 (Ndouble_plus_one a)).
-  apply Ndouble_plus_one_div2.  intro.  rewrite (H3 (Ndouble a)).
+  apply Ndouble_plus_one_div2.  intro.  rewrite (H3 (N.double a)).
   apply Ndouble_div2.
 Qed.
 
